\documentclass{article}
\input{eqn_abbr}
\usepackage{amsmath}
\usepackage{amssymb}
\usepackage{bm}
\usepackage{natbib}
\usepackage{hyperref}
\usepackage{breqn}

\begin{document}
\section{Approximate posteriors}
\begin{align}
\nonumber p(t_i=1|\cx_i,\cbeta)&=\int \delta(y_i>0)\cN(y_i|\cx_i\cbeta,1_)\,dy_i\\
\nonumber p(t_i=0|\cx_i,\cbeta)&=\int \delta(y_i<0)\cN(y_i|\cx_i\cbeta,1_)\,dy_i\\
p(t_i,y_i|\cx_i,\cbeta)&=\delta(y_i>0)^{t_i}\delta(y_i<0)^{1-t_i}\cN(y_i|\cx_i\cbeta,1)
\end{align}
Assume that $\cbeta$ has a non-informative prior of $\cN(\cbeta|\czero,1000\cI)$.

\begin{align}
p(\ct,\cy,\cbeta)&=\cN(\cbeta|\czero,1000\cI)\prod_{i=1}^{N}\delta(y_i>0)^{t_i}\delta(y_i<0)^{1-t_i}\cN(y_i|\cx_i\cbeta,1)
\end{align}

The approximate posterior on $\cbeta$ is shown below (\eqref{qb}). Let $\cX=\{\cx_1,\cx_2,...,\cx_n\}$.
\begin{align}
\nonumber\log q(\cbeta)&=\log \cN(\cbeta|\czero,1000\cI)-\chalf{}\csum(y_i-\cx_i^T\cbeta)^2\\
\nonumber&=-\chalf{}\clrbracket{\frac{\cbeta^T\cbeta}{1000}+\cbeta^T\cX\cX^T\cbeta-2\clrangle{\cy}^T\cX^T\cbeta}\\
\therefore q(\cbeta)&=\cN(\cmu,\cSigma)\\
\label{eq:qb}
\cSigma&=\clrbracket{\cX\cX^T+\frac{1}{1000}\cI}^{-1}\\
\cmu&=\cSigma\cX\clrangle{\cy}
\end{align}

\begin{align}
\nonumber\log q(y_i)&=t_i\log \delta(y_i>0)+(1-t_i)\log \delta(y_i<0)-\chalf{}(y_i-2y_i\cx_i^T\clrangle{\cbeta})\\
q(y_i)&=\cN_{t_i}(y_i|\cx_i^T\cmu,1)
\end{align}
Where $\cN_{t_i}$ is a left/right truncated normal distribution depending on $t_i=0$, $t_i=1$ respectively. The required expectations, $E(y_i)$, $E(y_i^2)$ are shown below.

\begin{align}
\nonumber C_i&=\begin{cases}
\int_{-\infty}^{0}\exp(-\chalf{}(y_i-\cx_i^T\cmu)^2)\,dy_i & t_i=0\\
\int_{0}^{\infty}\exp(-\chalf{}(y_i-\cx_i^T\cmu)^2)\,dy_i & t_i=1\\
\end{cases}\\
&=\begin{cases}
\sqrt{2\pi}\Phi(-\cx_i^T\cmu) & t_i=0\\
\sqrt{2\pi}(1-\Phi(-\cx_i^T\cmu)) & t_i=1\\
\end{cases}\\
\nonumber E(y_i)&=\begin{cases}
\int_{-\infty}^{0}y_i\frac{1}{C_i}\exp\clrbracket{-\chalf{}(y-\cx_i^T\cmu)^2}\,dy_i & t_i=0\\
\int_{0}^{\infty}y_i\frac{1}{C_i}\exp\clrbracket{-\chalf{}(y-\cx_i^T\cmu)^2}\,dy_i & t_i=1
\end{cases}\\
&=\begin{cases}
-\frac{1}{C_i}\exp\clrbracket{-\chalf{}(\cx_i^T\cmu)^2}+\cx_i^T\cmu & t_i=0\\
\frac{1}{C_i}\exp\clrbracket{-\chalf{}(\cx_i^T\cmu)^2}+\cx_i^T\cmu & t_i=1
\end{cases}\\
\nonumber E(y_i^2)&=\begin{cases}
-\frac{\cx_i^T\cmu\exp\clrbracket{-\chalf{}(\cx_i^T\cmu)^2}}{C_i}+(\cx_i^T\cmu)^2+1 & t_i=0\\
\frac{\cx_i^T\cmu\exp\clrbracket{-\chalf{}(\cx_i^T\cmu)^2}}{C_i}+(\cx_i^T\cmu)^2+1 & t_i=1
\end{cases}
\end{align}

\section{Log Likelihood}
In this section a lower bound for the log likelihood is obtained using the approximate distributions. Let $\delta_{t_i}(y_i)=\delta(y_i>0)^{t_i}\delta(y_i<0)^{1-t_i}$
\begin{align}
\nonumber \clrangle{\log p(\cy,\cbeta,\ct)}=&\csum\log\delta_{t_i}(y_i)\cN(y_i|\cx_i^T\cbeta,1)-\frac{d}{2}\log(2\pi\times1000)-\chalf{}\times\frac{1}{1000}\clrangle{\cbeta^T\cbeta}\\
\nonumber =&-\frac{N}{2}\log(2\pi)-\chalf{}\csum\clrbracket{ E(y_i^2)-2E(y_i)\cx_i^T\cmu+\cx_i^T\clrangle{\cbeta\cbeta^T}\cx_i}\\
\nonumber &-\frac{d}{2}\log(2\pi\times1000)-\chalf{}\times\frac{1}{1000}(\cmu^T\cmu+Tr(\cSigma))\\
\nonumber=&-\frac{N+d}{2}\log 2\pi-\frac{d}{2}\log 1000-\chalf{}\times\frac{1}{1000}(\cmu^T\cmu+Tr(\cSigma))\\
&-\chalf{}\csum\clrbracket{(-1)^{t_i}\frac{\cx_i^T\cmu\exp(-\chalf{}(\cx_i^T\cmu)^2)}{C_i}+1+\cx_i^T\cSigma\cx_i}
\end{align}

\begin{align}
\nonumber\clrangle{\log q(\cbeta)}=&-\chalf{}\log 2\pi|\cSigma|-\chalf{}(\cbeta-\cmu)^T\cSigma^{-1}(\cbeta-\cmu)\\
&=-\frac{d}{2}\log(2\pi)-\chalf{}\log|\cSigma|-\frac{d}{2}
\end{align}

\begin{align}
\nonumber\clrangle{\log q(y_i)}=&-\log C_i-\chalf{}\clrangle{(y_i^2-2\cx_i^T\cmu y_i+(\cx_i^T\cmu)^2)}\\
=&-\log C_i-\chalf{}\clrbracket{(-1)^{t_i}\frac{\cx_i^T\cmu\exp(-\chalf{}(\cx_i^T\cmu)^2)}{C_i}+1}
\end{align}
\appendix

\section{Expectations}
For $t_i=1$.
\begin{align}
\nonumber E(y^2)&=\int_{0}^{\infty}y^2\frac{1}{C_i}\exp\clrbracket{-\chalf{}(y-\mu)^2}\,dy \\
\nonumber \text{let }z=y-\mu \qquad E(y^2)&=\frac{1}{C_i}\int_{-\mu}^{\infty}z^2\exp\clrbracket{-\chalf{}z^2}dz+2\mu E(y)-\mu^2\\
\nonumber \text{let } u&=z\qquad dv=z\exp\clrbracket{-\chalf{}z^2}\\
\nonumber du&=dz \qquad v=-\exp\clrbracket{-\chalf{}z^2}\\
\nonumber \frac{1}{C_i}\int_{-\mu}^{\infty}z^2\exp\clrbracket{-\chalf{}z^2}dz &=\frac{-z\exp\clrbracket{-\chalf{}z^2}}{C_i}\Bigg|_{-\mu}^\infty+\frac{1}{C_i}\int_{-\mu}^{\infty}\exp\clrbracket{-\chalf{}z^2}\,dz\\
\nonumber &=-\frac{\mu\exp\clrbracket{-\chalf{}\mu^2}}{C_i}+1\\
\nonumber E(y^2)&=-\frac{\mu\exp\clrbracket{-\chalf{}\mu^2}}{C_i}+1+\mu^2+\frac{2\mu\exp\clrbracket{-\chalf{}\mu^2}}{C_i}\\
&=\frac{\mu\exp\clrbracket{-\chalf{}\mu^2}}{C_i}+\mu^2+1
\end{align}
Similarly for $t_i=0$,
\begin{align}
\nonumber E(y^2)&=\frac{\mu\exp\clrbracket{-\chalf{}\mu^2}}{C_i}+1+2\mu E(y)-\mu^2\\
&=-\frac{\mu\exp\clrbracket{-\chalf{}\mu^2}}{C_i}+\mu^2+1
\end{align}

\end{document}